Rewrite Repeated format to LengthDelimited format.

src/Narcissus/Examples/ProtobufSpec.v
@@ -1,6 +1,7 @@
 Require Import
         Coq.ZArith.BinInt
         Coq.Strings.String
+        Coq.Sets.Image
         Coq.Vectors.Vector
         Coq.omega.Omega
         Coq.Logic.Eqdep_dec.
@@ -47,222 +48,139 @@ Local Arguments NToWord : simpl never.
 Local Arguments wordToN : simpl never.
 Local Arguments pow2 : simpl never.
 Local Arguments weqb : simpl never.
+Local Arguments N.shiftl : simpl never.
+Local Arguments N.shiftr : simpl never.
+Local Arguments N.lor : simpl never.
+Local Arguments N.land : simpl never.
 
-Inductive PB_WireType : Set :=
-| PB_Varint : PB_WireType
-| PB_32bit : PB_WireType
-| PB_64bit : PB_WireType
-| PB_LengthDelimited : PB_WireType.
+Section LengthDelimited.
 
-Definition PB_WireType_denote (wty : PB_WireType) : N :=
-  match wty with
-  | PB_Varint => 0
-  | PB_32bit => 5
-  | PB_64bit => 1
-  | PB_LengthDelimited => 2
-  end.
+  Context {A : Type}.
+  Context {B : Type}.
+  Context {cache : Cache}.
+  Context {cacheAddNat : CacheAdd cache nat}.
+  Context {monoid : Monoid B}.
+  Context {monoidUnit : QueueMonoidOpt monoid bool}.
 
-Theorem PB_WireType_denote_3bits (wty : PB_WireType)
-  : N.lt (N.log2 (PB_WireType_denote wty)) 3%N.
-Proof.
-  destruct wty; easy.
-Qed.
+  Variable A_predicate : A -> Prop.
+  Variable A_predicate_rest : A -> B -> Prop.
+  Variable A_format : FormatM A B.
+  Variable A_decode : DecodeM A B.
+  Variable A_cache_inv : CacheDecode -> Prop.
+  Variable A_format_sz_eq : forall x b1 b2 ce1 ce1' ce2 ce2', A_format x ce1 ↝ (b1, ce1') ->
+                                                         A_format x ce2 ↝ (b2, ce2') ->
+                                                         bin_measure b1 = bin_measure b2.
+  Variable A_format_byte : forall d b ce ce', A_format d ce ↝ (b, ce') -> bin_measure b mod 8 = 0.
+  Variable A_decode_lt : forall b cd x b' cd', A_decode b cd = Some (x, b', cd') -> lt_B b' b.
+  Variable A_decode_correct : CorrectDecoder monoid A_predicate A_predicate_rest A_format A_decode A_cache_inv.
 
-Inductive PB_SingularType : Set :=
-| PB_fixed32 : PB_SingularType
-| PB_fixed64 : PB_SingularType
-| PB_int32 : PB_SingularType
-| PB_int64 : PB_SingularType
-(* | PB_sfixed32 : PB_SingularType *)
-(* | PB_sfixed64 : PB_SingularType *)
-(* | PB_bool : PB_SingularType *)
-(* | PB_string : PB_SingularType *)
-.
+  Definition PB_LengthDelimited_format
+    : FormatM (list A) B :=
+    (fun xs ce =>
+       `(b1, ce1) <- SizedList_format A_format xs ce;
+         `(b2, _) <- Varint_format (N.of_nat ((bin_measure b1) / 8)) ce;
+         ret (mappend b2 b1, ce1))%comp.
 
-Definition PB_SingularType_denote (sty : PB_SingularType) : Type :=
-   match sty with
-   | PB_fixed32 => word 32
-   | PB_fixed64 => word 64
-   (* :TODO: use word 32/64 later *)
-   (* :TODO: combinator for function composition? *)
-   | PB_int32 => N
-   | PB_int64 => N
-  end.
-
-Definition PB_SingularType_format (sty : PB_SingularType)
-  : FormatM (PB_SingularType_denote sty) ByteString :=
-  match sty with
-  | PB_fixed32 => format_word
-  | PB_fixed64 => format_word
-  | PB_int32 => Varint_format
-  | PB_int64 => Varint_format
-  end.
-
-Definition PB_SingularType_decoder
-           (sty : PB_SingularType)
-  : { decode : _ |
-      forall {P : CacheDecode -> Prop}
-        (P_OK : cache_inv_Property P (fun P => forall b cd, P cd -> P (addD cd b))),
-        CorrectDecoder _
-                       (fun _ => True)
-                       (fun _ _ => True)
-                       (PB_SingularType_format sty) decode P }.
-Proof.
-  let d := fill_ind_h
-             (PB_SingularType_rect
-                (fun sty => DecodeM (PB_SingularType_denote sty)
-                                 ByteString)) in
-  refine (exist _ (d sty) _).
-
-  intros; destruct sty; simpl;
-    repeat decode_step idtac.
-  all : apply Varint_decode_correct.
-  all : repeat decode_step idtac.
-Defined.
-
-Definition PB_SingularType_decode (sty : PB_SingularType) :=
-  Eval simpl in proj1_sig (PB_SingularType_decoder sty).
-
-(* :TODO: don't simply theorem and make them opaque. *)
-Definition PB_SingularType_decode_correct (sty : PB_SingularType) :=
-  Eval simpl in proj2_sig (PB_SingularType_decoder sty).
-
-Theorem PB_SingularType_format_sz_eq (sty : PB_SingularType)
-  : forall d b1 b2 ce1 ce1' ce2 ce2',
-    PB_SingularType_format sty d ce1 ↝ (b1, ce1') ->
-    PB_SingularType_format sty d ce2 ↝ (b2, ce2') ->
-    bin_measure b1 = bin_measure b2.
-Proof.
-  unfold PB_SingularType_format; intros; f_equal.
-  destruct sty;
-    repeat match goal with
-           | H : format_word _  _ ↝ _ |- _ => inversion H; subst; clear H
-           end;
-    auto; eapply Varint_format_eq; eauto.
-Qed.
-
-Theorem PB_SingularType_format_byte (sty : PB_SingularType)
-  : forall d b ce ce',
-    PB_SingularType_format sty d ce ↝ (b, ce') ->
-    bin_measure b mod 8 = 0.
-Proof.
-  unfold PB_SingularType_format.
-  destruct sty; intros;
-    solve [eapply format_word_byte; eauto; eauto |
-           eapply Varint_format_byte; eauto; eauto].
-Qed.
-
-Theorem PB_SingularType_decode_lt (sty : PB_SingularType)
-  : forall (b : ByteString) (cd : CacheDecode) (d : PB_SingularType_denote sty)
-      (b' : ByteString) (cd' : CacheDecode),
-    PB_SingularType_decode sty b cd = Some (d, b', cd') -> lt_B b' b.
-Proof.
-  intros.
-  destruct sty; simpl in *.
-  1-2 : unfold decode_word in H; eapply decode_word_lt; eauto.
-  all : eapply Varint_decode_lt; eauto.
-Qed.
-
-Definition PB_RepeatedType_denote (sty : PB_SingularType) : Type := list (PB_SingularType_denote sty).
-
-(* :Q: cache is funny. Is it a good idea to format sizedlist twice or ignore cache? *)
-Definition PB_RepeatedType_format (sty : PB_SingularType)
-  : FormatM (PB_RepeatedType_denote sty) ByteString :=
-  (fun xs ce =>
-     `(b1, ce1) <- SizedList_format (PB_SingularType_format sty) xs ce;
-       `(b2, _) <- Varint_format (N.of_nat ((bin_measure b1) / 8)) ce;
-       ret (mappend b2 b1, ce1))%comp.
-
-Definition PB_RepeatedType_decode (sty : PB_SingularType)
-  : DecodeM (PB_RepeatedType_denote sty) ByteString :=
+Definition PB_LengthDelimited_decode
+  : DecodeM (list A) B :=
   fun b cd =>
     `(sz, b1, cd1) <- (`(x, b1, cd1) <- Varint_decode b cd;
                         Some (N.to_nat x, b1, cd1));
-      SizedList_decode (PB_SingularType_decode sty)
-                       (PB_SingularType_decode_lt sty)
+      SizedList_decode A_decode A_decode_lt
                        (sz * 8) b1 cd.
 
 Local Arguments Nat.div : simpl never.
-Theorem PB_RepeatedType_decode_correct (sty : PB_SingularType)
-           {P : CacheDecode -> Prop}
-           (P_OK : cache_inv_Property P (fun P => forall b cd, P cd -> P (addD cd b)))
-  : CorrectDecoder _
-                   (fun _ => True)
-                   (fun _ _ => True)
-                   (PB_RepeatedType_format sty) (PB_RepeatedType_decode sty) P.
+Theorem PB_LengthDelimited_decode_correct
+        (A_cache_inv_OK : cache_inv_Property A_cache_inv (fun P => forall b cd, P cd -> P (addD cd b)))
+  : CorrectDecoder monoid
+                   (fun xs => forall x, In x xs -> A_predicate x)
+                   (SizedList_predicate_rest A_predicate_rest A_format)
+                   PB_LengthDelimited_format PB_LengthDelimited_decode A_cache_inv.
 Proof.
-  unfold PB_RepeatedType_format, PB_RepeatedType_decode.
+  unfold PB_LengthDelimited_format, PB_LengthDelimited_decode.
   split; intros. {
     computes_to_inv2.
-    edestruct (Varint_decode_correct (P:=P)) as [He _]; eauto.
-    edestruct He as [? [? [? ?]]]; eauto.
-    edestruct (SizedList_decode_correct _ _ _ _ _
-                                        (PB_SingularType_format_sz_eq sty)
-                                        (PB_SingularType_decode_lt sty)
-                                        (PB_SingularType_decode_correct sty P P_OK)) as [He' _].
-    clear H4 H5.
-    edestruct He' as [? [? [? ?]]]; try apply H2; eauto. intuition.
-    eapply SizedList_format_sz_eq. apply PB_SingularType_format_sz_eq. eauto. eauto.
-    apply SizedList_predicate_rest_True.
+    pose proof (Varint_decode_correct (P:=A_cache_inv)) as Hv.
+    eapply fun_compose_format_correct
+      with (predicate:=fun _ => True) (predicate_rest:=fun _ _ => True) (im:=fun _ => true)
+      in Hv.
+    edestruct Hv as [[? [? [? ?]]] _]; eauto. clear H4 H5.
+    edestruct (SizedList_decode_correct (A:=A)) as [[? [? [? ?]]] _]; try apply H2; eauto.
+    intuition. eapply SizedList_format_sz_eq; eauto.
     eexists. repeat split; eauto.
-    rewrite <- @mappend_assoc. rewrite H3.
-    simpl. rewrite Nnat.Nat2N.id.
+    rewrite <- mappend_assoc. rewrite H3.
+    simpl. rewrite Nat.mul_comm.
     assert (bin_measure b0 mod 8 = 0) as L. {
       eapply SizedList_format_byte; eauto.
-      apply PB_SingularType_format_byte.
     }
-    rewrite Nat.mul_comm. apply Nat.div_exact in L; auto.
-    simpl bin_measure in L. rewrite <- L.
-    simpl in H4. eauto.
+    apply Nat.div_exact in L; eauto. rewrite <- L; eauto.
+    all : auto.
+    intros. apply Nnat.Nat2N.id.
+    intros. simpl. econstructor. intuition. symmetry. apply Nnat.N2Nat.id.
   } {
     decode_opt_to_inv.
     subst.
-    edestruct (Varint_decode_correct (P:=P)) as [_ Hd]; eauto.
-    edestruct Hd as [? [? [? [? [? [? ?]]]]]]; eauto.
-    edestruct (SizedList_decode_correct _ _ _ _ _
-                                        (PB_SingularType_format_sz_eq sty)
-                                        (PB_SingularType_decode_lt sty)
-                                        (PB_SingularType_decode_correct sty P P_OK)) as [_ Hd'].
-    edestruct Hd' as [? [? [? [? [? [[? ?] ?]]]]]]; try apply H2; eauto.
+    pose proof (Varint_decode_correct (P:=A_cache_inv)) as Hv.
+    eapply fun_compose_format_correct
+      with (predicate:=fun _ => True) (predicate_rest:=fun _ _ => True) (im:=fun _ => true)
+      in Hv.
+    edestruct Hv as [_ [? [? [? [? [? [? ?]]]]]]]; eauto.
+    rewrite H1. simpl. reflexivity.
+    edestruct (SizedList_decode_correct (A:=A)) as [_ [? [? [? [? [? [[? ?] ?]]]]]]]; try apply H2; eauto.
     split; eauto.
     eexists _, _. repeat split; eauto.
-    computes_to_econstructor. eauto.
     computes_to_econstructor; eauto.
-    apply H11 in H9. simpl fst. rewrite H9. rewrite Nat.div_mul by auto.
-    rewrite Nnat.N2Nat.id. eauto.
+    computes_to_econstructor; eauto.
+    apply H11 in H9. simpl fst. rewrite H9. rewrite Nat.div_mul by auto. eauto.
     simpl fst. rewrite <- mappend_assoc. subst. reflexivity.
+    all : auto.
+    intros. apply Nnat.Nat2N.id.
+    intros. simpl. econstructor. intuition. symmetry. apply Nnat.N2Nat.id.
   }
 Qed.
 
-Theorem PB_RepeatedType_format_sz_eq (sty : PB_SingularType)
+Theorem PB_LengthDelimited_format_sz_eq
   : forall d b1 b2 ce1 ce1' ce2 ce2',
-    PB_RepeatedType_format sty d ce1 ↝ (b1, ce1') ->
-    PB_RepeatedType_format sty d ce2 ↝ (b2, ce2') ->
+    PB_LengthDelimited_format d ce1 ↝ (b1, ce1') ->
+    PB_LengthDelimited_format d ce2 ↝ (b2, ce2') ->
     bin_measure b1 = bin_measure b2.
 Proof.
-  unfold PB_RepeatedType_format. intros.
-  computes_to_inv2. rewrite !@mappend_measure.
+  unfold PB_LengthDelimited_format. intros.
+  computes_to_inv2. rewrite !mappend_measure.
   assert (bin_measure b4 = bin_measure b0). {
     eapply SizedList_format_sz_eq; eauto.
-    apply PB_SingularType_format_sz_eq.
   }
   rewrite H1 in *.
   erewrite Varint_format_sz_eq; eauto.
 Qed.
 
-Theorem PB_RepeatedType_format_byte (sty : PB_SingularType)
+Theorem PB_LengthDelimited_decode_lt
+  : forall b cd d b' cd',
+    PB_LengthDelimited_decode b cd = Some (d, b', cd') -> lt_B b' b.
+Proof.
+  unfold PB_LengthDelimited_decode. intros.
+  decode_opt_to_inv.
+  apply Varint_decode_lt in H.
+  apply SizedList_decode_le in H0.
+  unfold lt_B, le_B in *. subst. omega.
+Qed.
+
+End LengthDelimited.
+
+Theorem PB_LengthDelimited_format_byte
+        {A : Type} (A_format : FormatM A ByteString)
+        (A_format_byte : forall d b ce ce', A_format d ce ↝ (b, ce') -> bin_measure b mod 8 = 0)
   : forall d b ce ce',
-    PB_RepeatedType_format sty d ce ↝ (b, ce') ->
+    PB_LengthDelimited_format A_format d ce ↝ (b, ce') ->
     bin_measure b mod 8 = 0.
 Proof.
-  unfold PB_RepeatedType_format.
+  unfold PB_LengthDelimited_format.
   intros. computes_to_inv2.
   rewrite @mappend_measure.
   rewrite <- Nat.add_mod_idemp_l by auto.
   rewrite <- Nat.add_mod_idemp_r by auto.
   erewrite Varint_format_byte; eauto.
   erewrite SizedList_format_byte; eauto.
-  apply PB_SingularType_format_byte.
 Qed.
 
 Inductive PB_Type : Set :=
